src/DirTree.v
@@ -2165,6 +2165,8 @@ Module DIRTREE.
 
   Hint Extern 1 ({{_}} progseq (read _ _ _ _) _) => apply read_ok : prog.
   Hint Extern 1 ({{_}} progseq (write _ _ _ _ _) _) => apply write_ok : prog.
+  Hint Extern 1 ({{_}} progseq (update_bytes _ _ _ _ _) _) => apply update_bytes_ok : prog.
+  Hint Extern 1 ({{_}} progseq (append _ _ _ _ _) _) => apply append_ok : prog.
   Hint Extern 1 ({{_}} progseq (truncate _ _ _ _) _) => apply truncate_ok : prog.
   Hint Extern 1 ({{_}} progseq (getlen _ _ _) _) => apply getlen_ok : prog.
   Hint Extern 1 ({{_}} progseq (getattr _ _ _) _) => apply getattr_ok : prog.
